td progress

common/array.v
@@ -1,7 +1,8 @@
+Require Import Program.
 Require Import Omega.
 Require Import Braun.common.log.
 Require Import Braun.common.le_util.
-Require Import List.
+Require Import Arith Arith.Even Arith.Div2 List.
 
 Fixpoint man_time n : nat :=
   match n with
@@ -37,3 +38,63 @@ Proof.
   apply cl_log_monotone.
 Qed.
 Hint Resolve man_time_nlogn.
+
+(* this is http://oeis.org/A001855 *)
+Program Fixpoint mat_time n {measure n} :=
+  match n with
+    | O => 0
+    | S n' =>
+      mat_time (div2 n) + mat_time (div2 n') + n
+  end.
+
+Lemma mat_time_Sn : 
+  forall n',
+    mat_time (S n') = 
+    mat_time (div2 (S n')) +
+    mat_time (div2 n') +
+    (S n').
+Proof.
+  intros.
+  WfExtensionality.unfold_sub 
+    mat_time
+    (mat_time (S n')).
+  auto.
+Qed.
+
+Lemma mat_time_Sn_cl_log : 
+  forall n : nat,
+    mat_time (S n) = mat_time n + cl_log (S n).
+Proof.
+  apply (well_founded_ind
+           lt_wf
+           (fun n => mat_time (S n) = mat_time n + cl_log (S n))).
+
+  intros n IHn.
+  
+  destruct n.
+  compute;reflexivity.
+
+  rewrite mat_time_Sn.
+
+  replace (div2 (S (S n))) with (S (div2 n));[|unfold div2;reflexivity].
+
+  rewrite IHn;auto.
+
+  replace (cl_log (S (S n))) with (S (cl_log (div2 (S (S n)))));
+    [|symmetry;apply cl_log_div2'].
+  
+  rewrite mat_time_Sn.
+  
+  replace (div2 (S (S n))) with (S (div2 n));[|unfold div2;reflexivity].
+
+  omega.
+Qed.
+
+Lemma rt_naive_same_as_mat_time :
+  forall n, mat_time n = man_time n.
+Proof.
+  induction n.
+  auto.
+  
+  simpl; rewrite <- IHn; apply mat_time_Sn_cl_log; auto.
+Qed.
