logical/make_array_td.v
@@ -198,28 +198,6 @@ Proof.
 Qed.
 Hint Resolve MakeArrayTDR_correct.
 
-(* this is http://oeis.org/A001855 *)
-Program Fixpoint mat_time n {measure n} :=
-  match n with
-    | O => 0
-    | S n' =>
-      mat_time (div2 n) + mat_time (div2 n') + n
-  end.
-
-Lemma mat_time_Sn : 
-  forall n',
-    mat_time (S n') = 
-    mat_time (div2 (S n')) +
-    mat_time (div2 n') +
-    (S n').
-Proof.
-  intros.
-  WfExtensionality.unfold_sub 
-    mat_time
-    (mat_time (S n')).
-  auto.
-Qed.
-
 Lemma MakeArrayTDR_exact_time :
   forall A xs (bt:@bin_tree A) t,
     MakeArrayTDR xs bt t ->
@@ -326,41 +304,4 @@ Proof.
   omega.
 
   apply mat_time_nlogn.
-Qed.
-
-Lemma mat_time_Sn_cl_log : 
-  forall n : nat,
-    mat_time (S n) = mat_time n + cl_log (S n).
-  apply (well_founded_ind
-           lt_wf
-           (fun n => mat_time (S n) = mat_time n + cl_log (S n))).
-
-  intros n IHn.
-  
-  destruct n.
-  compute;reflexivity.
-
-  rewrite mat_time_Sn.
-
-  replace (div2 (S (S n))) with (S (div2 n));[|unfold div2;reflexivity].
-
-  rewrite IHn;auto.
-
-  replace (cl_log (S (S n))) with (S (cl_log (div2 (S (S n)))));
-    [|symmetry;apply cl_log_div2'].
-  
-  rewrite mat_time_Sn.
-  
-  replace (div2 (S (S n))) with (S (div2 n));[|unfold div2;reflexivity].
-
-  omega.
-Qed.
-
-Lemma rt_naive_same_as_mat_time :
-  forall n, mat_time n = man_time n.
-Proof.
-  induction n.
-  auto.
-  
-  simpl; rewrite <- IHn; apply mat_time_Sn_cl_log; auto.
 Qed.
