tmonad/make_array_td.v
@@ -1,0 +1,55 @@
+Require Import Braun.tmonad.monad.
+Require Import Braun.tmonad.insert.
+
+Require Import Braun.logical.sequence.
+Require Import Braun.logical.list_util.
+
+Require Import Braun.common.braun.
+Require Import Braun.common.array.
+Require Import Braun.common.util.
+Require Import Braun.common.log.
+
+Program Fixpoint unravel (A:Set) (xs:list A) :
+  {! eo !:! ((list A) * (list A))
+     !<! c !>!
+     xs = interleave (fst eo) (snd eo) 
+   /\ c = length xs !} :=
+  match xs with
+    | nil =>
+      <== (nil, nil)
+    | (cons x xs') =>
+      moe <- unravel A xs' ;
+      ++ ;
+      <== ( (cons x (snd moe)), (fst moe) )
+  end.
+
+Next Obligation.
+  simpl. rename l into e. rename l0 into o.
+  split; try omega.
+  apply interleave_case2.
+Qed.
+
+Program Fixpoint make_array_td (A:Set) xs {measure (length xs)} :
+  {! b !:! @bin_tree A
+     !<! c !>!
+     let n := length xs in
+     Braun b n
+     /\ c = mat_time n
+     /\ SequenceR b xs !} :=
+  match xs with
+    | nil      =>
+      <== bt_mt
+    | (cons x xs') =>
+      eo <- unravel A xs' ;
+      oa <- make_array_td A (snd eo) ;
+      ea <- make_array_td A (fst eo) ;
+      <== (bt_node x oa ea)
+  end.
+
+Obligations.
+
+(* XXX This is very interesting, Obligations 2 and 3 are wrong because
+they drop the relation between eo and the argument, so I can't use
+theorems about interleave. *)
+
+Admit Obligations.
